pr/320/head/ts/student/lean/TS.lean
@@ -3,3 +3,4 @@ import TS.Slang
 import TS.Smallstep
 import TS.Types
 import TS.Stlc
+import TS.StlcProp
